Define pointable

src/sequential/NALoc.v
@@ -141,14 +141,389 @@ Lemma sim_local_read_na
       (NA: Ordering.le ord_src Ordering.na)
       (CONS: Local.promise_consistent lc2_tgt)
   :
-    (exists released_src lc2_src,
-        (<<REL: View.opt_le released_src released_tgt>>) /\
-        (<<STEP_SRC: Local.read_step lc1_src mem1_src loc ts val released_src ord_src lc2_src>>) /\
-        (<<LC: lc2_src = lc1_src>>)) \/
-    (<<STEP_SRC: Local.racy_read_step lc1_src mem1_src loc ts val ord_src>>).
+    (<<LOCAL2: JSim.sim_local views lc1_src lc2_tgt>>) /\
+    ((exists released_src lc2_src,
+         (<<REL: View.opt_le released_src released_tgt>>) /\
+         (<<STEP_SRC: Local.read_step lc1_src mem1_src loc ts val released_src ord_src lc2_src>>) /\
+         (<<LC: lc2_src = lc1_src>>)) \/
+     (<<STEP_SRC: Local.racy_read_step lc1_src mem1_src loc ts val ord_src>>)).
 Proof.
+  splits.
+  { inv LOCAL1. inv STEP_TGT. econs; eauto. ss.
+    etrans; eauto. eapply TViewFacts.read_tview_incr; eauto.
+  }
   exploit sim_local_read_na_aux; eauto. i. des; eauto.
   exploit read_step_plain_cur;
     try exact STEP_SRC; try apply WF1_SRC; eauto. i. subst.
   left. esplits; eauto.
 Qed.
+
+Require Import DelayedStep.
+Require Import NoMix.
+Require Import gSimAux.
+
+Section POINTABLE.
+  Variable loc_na: Loc.t -> Prop.
+
+  Variable msgs: Messages.t.
+  Hypothesis MSGSBOT: forall loc, msgs loc Time.bot Time.bot Message.elt.
+
+  Definition pointable_timemap (tm: TimeMap.t): Prop :=
+    forall loc (NA: loc_na loc),
+    exists from val released, msgs loc (tm loc) from (Message.concrete val released).
+
+  Lemma pointable_timemap_join tm0 tm1
+        (TM0: pointable_timemap tm0)
+        (TM1: pointable_timemap tm1)
+    :
+      pointable_timemap (TimeMap.join tm0 tm1).
+  Proof.
+    ii. unfold TimeMap.join, Time.join.  des_ifs.
+    { eapply TM1; eauto. }
+    { eapply TM0; eauto. }
+  Qed.
+
+  Lemma pointable_timemap_bot
+    :
+      pointable_timemap TimeMap.bot.
+  Proof.
+    ii. esplits. eapply MSGSBOT.
+  Qed.
+
+  Lemma pointable_timemap_singleton loc ts
+        (POINTED: forall (NA: loc_na loc), exists from val released, msgs loc ts from (Message.concrete val released))
+    :
+      pointable_timemap (TimeMap.singleton loc ts).
+  Proof.
+    ii. unfold TimeMap.singleton. setoid_rewrite LocFun.add_spec. des_ifs.
+    { eapply POINTED; eauto. }
+    { esplits. rewrite LocFun.init_spec. eapply MSGSBOT. }
+  Qed.
+
+  Record pointable_view (vw: View.t): Prop :=
+    { pointable_pln: pointable_timemap vw.(View.pln);
+      pointable_rlx: pointable_timemap vw.(View.rlx);
+    }.
+
+  Lemma pointable_view_join vw0 vw1
+        (VW0: pointable_view vw0)
+        (VW1: pointable_view vw1)
+    :
+      pointable_view (View.join vw0 vw1).
+  Proof.
+    econs; ss.
+    { eapply pointable_timemap_join; eauto.
+      { eapply VW0. }
+      { eapply VW1. }
+    }
+    { eapply pointable_timemap_join; eauto.
+      { eapply VW0. }
+      { eapply VW1. }
+    }
+  Qed.
+
+  Lemma pointable_view_bot
+    :
+      pointable_view View.bot.
+  Proof.
+    econs.
+    { eapply pointable_timemap_bot; eauto. }
+    { eapply pointable_timemap_bot; eauto. }
+  Qed.
+
+  Lemma pointable_view_singleton_ur loc ts
+        (POINTED: forall (NA: loc_na loc), exists from val released, msgs loc ts from (Message.concrete val released))
+    :
+      pointable_view (View.singleton_ur loc ts).
+  Proof.
+    econs; ss.
+    { eapply pointable_timemap_singleton; eauto. }
+    { eapply pointable_timemap_singleton; eauto. }
+  Qed.
+
+  Lemma pointable_view_singleton_rw loc ts
+        (POINTED: forall (NA: loc_na loc), exists from val released, msgs loc ts from (Message.concrete val released))
+    :
+      pointable_view (View.singleton_rw loc ts).
+  Proof.
+    econs; ss.
+    { eapply pointable_timemap_bot; eauto. }
+    { eapply pointable_timemap_singleton; eauto. }
+  Qed.
+
+  Lemma pointable_view_singleton_ur_if loc ts cond
+        (POINTED: forall (NA: loc_na loc), exists from val released, msgs loc ts from (Message.concrete val released))
+    :
+      pointable_view (View.singleton_ur_if cond loc ts).
+  Proof.
+    destruct cond; ss.
+    { eapply pointable_view_singleton_ur; eauto. }
+    { eapply pointable_view_singleton_rw; eauto. }
+  Qed.
+
+  Variant pointable_opt_view: forall (vw: option View.t), Prop :=
+  | pointable_opt_view_some
+      vw
+      (VW: pointable_view vw)
+    :
+      pointable_opt_view (Some vw)
+  | pointable_opt_view_nond
+    :
+      pointable_opt_view None
+  .
+
+  Lemma pointable_unwrap vw
+        (VW: pointable_opt_view vw)
+    :
+      pointable_view (View.unwrap vw).
+  Proof.
+    inv VW; auto. eapply pointable_view_bot; eauto.
+  Qed.
+
+  Record pointable_tview (tvw: TView.t): Prop :=
+    { pointable_rel: forall loc, pointable_view (tvw.(TView.rel) loc);
+      pointable_cur: pointable_view tvw.(TView.cur);
+      pointable_acq: pointable_view tvw.(TView.acq);
+    }.
+
+  Lemma pointable_read_tview tvw loc ts released ord
+        (TVW: pointable_tview tvw)
+        (POINTED: forall (NA: loc_na loc), exists from val released, msgs loc ts from (Message.concrete val released))
+        (RELEASED: pointable_opt_view released)
+    :
+      pointable_tview (TView.read_tview tvw loc ts released ord).
+  Proof.
+    econs; ss.
+    { i. eapply TVW. }
+    { des_ifs.
+      { eapply pointable_view_join; eauto.
+        { eapply pointable_view_join.
+          { eapply TVW. }
+          { eapply pointable_view_singleton_ur_if; eauto. }
+        }
+        { eapply pointable_unwrap; eauto. }
+      }
+      { eapply pointable_view_join; eauto.
+        { eapply pointable_view_join.
+          { eapply TVW. }
+          { eapply pointable_view_singleton_ur_if; eauto. }
+        }
+        { eapply pointable_view_bot; eauto. }
+      }
+    }
+    { des_ifs.
+      { eapply pointable_view_join; eauto.
+        { eapply pointable_view_join.
+          { eapply TVW. }
+          { eapply pointable_view_singleton_ur_if; eauto. }
+        }
+        { eapply pointable_unwrap; eauto. }
+      }
+      { eapply pointable_view_join; eauto.
+        { eapply pointable_view_join.
+          { eapply TVW. }
+          { eapply pointable_view_singleton_ur_if; eauto. }
+        }
+        { eapply pointable_view_bot; eauto. }
+      }
+    }
+  Qed.
+
+  Lemma pointable_write_tview tvw sc loc ts ord
+        (TVW: pointable_tview tvw)
+        (POINTED: forall (NA: loc_na loc), exists from val released, msgs loc ts from (Message.concrete val released))
+    :
+      pointable_tview (TView.write_tview tvw sc loc ts ord).
+  Proof.
+    econs; ss.
+    { i. setoid_rewrite LocFun.add_spec. des_ifs.
+      { eapply pointable_view_join; eauto.
+        { eapply TVW. }
+        { eapply pointable_view_singleton_ur; eauto. }
+      }
+      { eapply pointable_view_join; eauto.
+        { eapply TVW. }
+        { eapply pointable_view_singleton_ur; eauto. }
+      }
+      { eapply TVW. }
+    }
+    { eapply pointable_view_join; eauto.
+      { eapply TVW. }
+      { eapply pointable_view_singleton_ur; eauto. }
+    }
+    { eapply pointable_view_join; eauto.
+      { eapply TVW. }
+      { eapply pointable_view_singleton_ur; eauto. }
+    }
+  Qed.
+
+  Lemma pointable_read_fence_tview tvw ord
+        (TVW: pointable_tview tvw)
+    :
+      pointable_tview (TView.read_fence_tview tvw ord).
+  Proof.
+    econs; ss.
+    { i. eapply TVW. }
+    { des_ifs.
+      { eapply TVW. }
+      { eapply TVW. }
+    }
+    { eapply TVW. }
+  Qed.
+
+  Lemma pointable_write_fence_sc tvw sc ord
+        (TVW: pointable_tview tvw)
+        (SC: pointable_timemap sc)
+    :
+      pointable_timemap (TView.write_fence_sc tvw sc ord).
+  Proof.
+    unfold TView.write_fence_sc. des_ifs.
+    eapply pointable_timemap_join; eauto. eapply TVW.
+  Qed.
+
+  Lemma pointable_write_fence_tview tvw sc ord
+        (TVW: pointable_tview tvw)
+        (SC: pointable_timemap sc)
+    :
+      pointable_tview (TView.write_fence_tview tvw sc ord).
+  Proof.
+    econs; ss.
+    { i. des_ifs; ss.
+      { econs; eapply pointable_write_fence_sc; eauto. }
+      { eapply TVW. }
+      { eapply TVW. }
+    }
+    { des_ifs; ss.
+      { econs; eapply pointable_write_fence_sc; eauto. }
+      { eapply TVW. }
+    }
+    { des_ifs; ss.
+      { eapply pointable_view_join.
+        { eapply TVW. }
+        { econs; eapply pointable_write_fence_sc; eauto. }
+      }
+      { eapply pointable_view_join.
+        { eapply TVW. }
+        { eapply pointable_view_bot. }
+      }
+    }
+  Qed.
+
+  Lemma pointable_write_released tvw sc loc ts releasedm ord
+        (TVW: pointable_tview tvw)
+        (POINTED: forall (NA: loc_na loc), exists from val released, msgs loc ts from (Message.concrete val released))
+        (RELEASED: pointable_opt_view releasedm)
+    :
+      pointable_opt_view (TView.write_released tvw sc loc ts releasedm ord).
+  Proof.
+    unfold TView.write_released. des_if; econs.
+    eapply pointable_view_join.
+    { eapply pointable_unwrap; eauto. }
+    { eapply pointable_write_tview; eauto. }
+  Qed.
+
+  Variant pointable_message: forall (msg: Message.t), Prop :=
+  | pointable_concrete
+      val released
+      (RELEASED: pointable_opt_view released)
+    :
+      pointable_message (Message.concrete val released)
+  | pointable_undef
+    :
+      pointable_message Message.undef
+  | pointable_reserve
+    :
+      pointable_message Message.reserve
+  .
+
+  Definition pointable_memory (mem: Memory.t): Prop :=
+    forall loc (AT: ~ loc_na loc) from to val released
+           (GET: Memory.get loc to mem = Some (from, Message.concrete val released)),
+      pointable_opt_view released.
+
+  Lemma pointable_write prom0 mem0 loc from to msg prom1 mem1 kind
+        (WRITE: Memory.write prom0 mem0 loc from to msg prom1 mem1 kind)
+        (MEM: pointable_memory mem0)
+        (MSG: forall (AT: ~ loc_na loc), pointable_message msg)
+    :
+      pointable_memory mem1.
+  Proof.
+    inv WRITE. inv PROMISE.
+    { ii. erewrite Memory.add_o in GET; eauto. des_ifs.
+      { ss. des; clarify. specialize (MSG AT). inv MSG. eauto. }
+      { eapply MEM; eauto. }
+    }
+    { ii. erewrite Memory.split_o in GET; eauto. des_ifs.
+      { ss. des; clarify. specialize (MSG AT). inv MSG. eauto. }
+      { ss. des; clarify. eapply Memory.split_get0 in MEM0. des.
+        eapply MEM; eauto.
+      }
+      { eapply MEM; eauto. }
+    }
+    { ii. erewrite Memory.lower_o in GET; eauto. des_ifs.
+      { ss. des; clarify. specialize (MSG AT). inv MSG. eauto. }
+      { eapply MEM; eauto. }
+    }
+    { ii. erewrite Memory.remove_o in GET; eauto. des_ifs.
+      eapply MEM; eauto.
+    }
+  Qed.
+
+  Lemma pointable_write_na ts prom0 mem0 loc from to val prom1 mem1 msgs0 kinds kind
+        (WRITE: Memory.write_na ts prom0 mem0 loc from to val prom1 mem1 msgs0 kinds kind)
+        (MEM: pointable_memory mem0)
+    :
+      pointable_memory mem1.
+  Proof.
+    revert MEM. induction WRITE; i.
+    { eapply pointable_write; eauto. econs; eauto. econs. }
+    { eapply IHWRITE. eapply pointable_write; eauto.
+      red in MSG_EX. des; clarify; econs; eauto. econs.
+    }
+  Qed.
+
+  Definition pointable_views (views: Loc.t -> Time.t -> list View.t): Prop :=
+    forall loc (AT: ~ loc_na loc) ts,
+      List.Forall pointable_view (views loc ts).
+
+  Lemma pointable_joined_opt_view views released
+        (JOINED: joined_opt_view views released)
+        (VIEWS: List.Forall pointable_view views)
+    :
+      pointable_opt_view released.
+  Proof.
+    inv JOINED; econs.
+    revert VIEWS. induction JOINED0; i.
+    { eapply pointable_view_bot; eauto. }
+    { eapply pointable_view_join; eauto.
+      eapply List.Forall_forall in VIEW; eauto.
+    }
+  Qed.
+
+  Lemma pointable_views_incr tvw (views1 views2: Loc.t -> Time.t -> list View.t)
+        (VIEWS: pointable_views views1)
+        (TVIEW: pointable_tview tvw)
+        (VIEWSLE: forall loc ts (NEQ: views2 loc ts <> views1 loc ts),
+            (<<NIL: views1 loc ts = []>>) /\
+            exists from,
+              (<<VIEW: views2 loc ts = (View.join (tvw.(TView.rel) loc) (View.singleton_ur loc ts))
+                                         ::(all_join_views (View.singleton_ur loc ts) (views1 loc from))>>))
+    :
+      pointable_views views2.
+  Proof.
+    ii. destruct (classic (views2 loc ts = views1 loc ts)).
+    { rewrite H. eapply VIEWS; eauto. }
+    { hexploit VIEWSLE; eauto. i. des. rewrite VIEW. econs.
+      { eapply pointable_view_join.
+        { eapply TVIEW. }
+        { eapply pointable_view_singleton_ur; eauto. i. ss. }
+      }
+      { unfold all_join_views. eapply list_map_forall.
+        { eapply VIEWS; eauto. }
+        { i. eapply pointable_view_join; auto.
+          eapply pointable_view_singleton_ur; eauto. i. ss.
+        }
+      }
+    }
+  Qed.
+End POINTABLE.
